updated after btree restructuring

verif/indices/ordered_interface.v
@@ -1,23 +1,14 @@
 Require Import VST.floyd.functional_base VST.floyd.proofauto.
 Require Import Coq.ZArith.BinInt.
-Require Import unordered_flat.
+Require Import indices.unordered_flat.
 Require Import VST.floyd.library.
-Require Import definitions.
+Require Import indices.definitions.
 
 Infix ">=" := Z.geb : Z_scope.
 Infix "<=" := Z.leb : Z_scope.
 Infix "<" := Z.ltb: Z_scope.
 Infix ">" := Z.gtb: Z_scope.
 Infix "=" := Z.eqb: Z_scope.
-
-Definition get_cursor_unordered {key: Type} {eq_dec: EqDec key} (k0: key) (l: flat key): Z :=
-  (fix f l i :=
-     match l with
-     | nil => i
-     | (k, v) :: tl =>
-       if eq_dec k k0 then i
-       else f tl (i + 1)
-     end) (elements l) 0.
 
 Module OrderedIndex.
 
@@ -28,204 +19,172 @@ Record index :=
     default_key: Inhabitant key;
     key_repr: share -> key -> val -> mpred;
     
-    value := sig is_pointer_or_null;
+    value := val;
     default_value: Inhabitant value;
 
     t: Type;
     t_repr: share -> t -> val -> mpred;
-
-    kvpair := (key * value)%type;
     
-    cursor := (t * Z)%type;
-    cursor_repr: cursor -> val -> mpred;
+    cursor : Type;
+    cursor_repr: cursor -> val -> Z -> mpred;
+    cursor_type: type;
 
-    flatten: t -> flat key;
+    (* helpers *)
+    valid_cursor: cursor -> bool;
+
+    (* interface *)
     
-    cardinality: t -> Z := 
-        fun m => Zlength (elements (flatten m));
+    cardinality: t -> Z;
 
-    (* returns cursor that points to some key in the index
-        or to the end if no key found *)
-    get_cursor: t -> key -> cursor := 
-        fun m k => (m, get_cursor_unordered k (flatten m));
+    move_to_key: cursor -> key -> cursor;
 
-    (* returns a valid kvpair from the list or None if cursor invalid
-        or reached end of structure *)
-    get_pair: cursor -> option kvpair :=
-        fun '(m, c) => let lst := elements (flatten m) in
-                              if c >= (Zlength lst) then None
-                              else if c < 0 then None
-                              else Some (Znth c (elements (flatten m)));
+    move_to_next: cursor -> cursor;
 
-    (* moves cursor to next position *)
-    move_to_next: cursor -> cursor:= 
-        fun '(m, c) => let newcur := (m, (c + 1)) in
-                              let lst := elements (flatten m) in
-                              let lastcur := (Zlength lst - 1) in
-                              (* if moving past end, return cursor pointing to end *)
-                              if (c + 1) > (Zlength lst) then (m, lastcur)
-                              (* if cursor before start, return cursor pointing to start *)
-                              else if (c + 1) <= 0 then (m, 0) else newcur;
+    move_to_previous: cursor -> cursor;
 
-    (* moves cursor to prev position*)
-    move_to_previous: cursor -> cursor := 
-        fun '(m, c) => let newcur := (m, (c - 1)) in
-                              let lst := elements (flatten m) in
-                              let lastcur := (Zlength lst - 1) in
-                              (* if cursor past end, return last cursor *)
-                              if (c - 1) >= (Zlength lst) then (m, lastcur)
-                              (* if cursor before start, return cursor pointing to start *)
-                              else if (c -1) < 0 then (m, 0) else newcur;
+    move_to_first: cursor -> cursor;
 
-    move_to_first: t -> cursor := fun m => (m, 0);
+    move_to_last: cursor -> cursor;
 
-    move_to_last: t -> cursor := 
-        fun m => let lst := (elements (flatten m)) in (m, (Zlength lst - 1));
-
-    insert: cursor -> kvpair -> cursor;
-
-    delete: cursor -> key -> cursor;
-
-    (* move to key operation *)
-
-    lookup: t -> key -> value :=
-      fun m k => let kv := get_pair (move_to_next (get_cursor m k)) in
-                         match kv with
-                         | None => nullV
-                         | Some (k0, v0) => if eq_dec_key k0 k then v0 else nullV
-                         end;
   }.
+
+(* ================= VERIFIED =============== *)
+
+(* takes t, returns cursor pointing to 0 *)
+Definition move_to_next_spec 
+  (oi: OrderedIndex.index): funspec :=
+  WITH p: val, cur: oi.(cursor), numrec: Z
+  PRE [ 1%positive OF tptr oi.(cursor_type)]
+    PROP()
+    LOCAL(temp 1%positive p)
+    SEP(oi.(cursor_repr) cur p numrec)
+  POST [tvoid]
+    PROP()
+    LOCAL()
+    SEP(oi.(cursor_repr) (oi.(move_to_next) cur) p numrec).
+
+
+(*
+Definition create_index_spec 
+  (oi: OrderedIndex.index): funspec :=
+  WITH gv: globals, sh: share
+  PRE [ ]
+    PROP()
+    LOCAL(gvars gv)
+    SEP(mem_mgr gv)
+  POST [tptr tvoid]
+    EX p: val, EX m: oi.(t),
+    PROP( oi.(cardinality) m = 0 )
+    LOCAL(temp ret_temp p)
+    SEP(oi.(t_repr) sh m p; mem_mgr gv).
+
+Definition create_cursor_spec 
+  (oi: OrderedIndex.index): funspec :=
+  WITH gv: globals, sh: share, m: oi.(t), p: val
+  PRE [1 OF tptr tvoid ]
+    PROP()
+    LOCAL(gvars gv)
+    SEP(mem_mgr gv; oi.(t_repr) sh m p)
+  POST [tptr tvoid]
+    EX q: val, EX cur: oi.(cursor),
+    PROP ( )
+    LOCAL(temp ret_temp p)
+    SEP(oi.(cursor_repr) cur q; mem_mgr gv).
 
 (* takes t, returns Z *)
 Definition cardinality_spec 
   (oi: OrderedIndex.index): funspec :=
   WITH sh: share, p: val, m: oi.(t)
-  PRE [ 1%positive OF tptr tvoid]
+  PRE [ 1 OF tptr tvoid]
     PROP()
-    LOCAL( temp 1%positive p)
+    LOCAL( temp 1 p)
     SEP(oi.(t_repr) sh m p)
-  POST [size_t]
+  POST [tulong]
     PROP()
-    LOCAL(temp ret_temp (Vptrofs (Ptrofs.repr (Zlength (elements(oi.(flatten) m))))))
+    LOCAL(temp ret_temp (Vptrofs (Ptrofs.repr (oi.(cardinality) m))))
     SEP(oi.(t_repr) sh m p).
 
-(* takes t, k, returns cursor *)
-(* for now, for simplicity, returns pointer to cursor *)
 Definition get_cursor_spec 
   (oi: OrderedIndex.index): funspec :=
   WITH gv: globals, sh: share, p: val, q: val, m: oi.(t), k: oi.(key)
   PRE [ 1%positive OF tptr tvoid, 2%positive OF tptr tvoid]
     PROP()
-    LOCAL(temp 1%positive p; temp 2%positive q)
+    LOCAL(gvars gv; temp 1%positive p; temp 2%positive q)
     SEP(mem_mgr gv; oi.(t_repr) sh m p *  oi.(key_repr) sh k q)
   POST [tptr tvoid]
     EX r: val, EX c: oi.(cursor),
     PROP()
     LOCAL(temp ret_temp r)
-    SEP(mem_mgr gv; oi.(t_repr) sh m p *  oi.(key_repr) sh k q * oi.(cursor_repr) c r).
-
-(* change these to reflect move_to_next, move_to_previous, add get_pair
-Definition get_next_spec 
-  (oi: OrderedIndex.index): funspec :=
-  WITH sh: share, p: val, mc: oi.(cursor)
-  PRE [ 1%positive OF tptr tvoid]
-    PROP()
-    LOCAL( temp 1%positive p)
-    SEP(oi.(cursor_repr) mc p)
-  POST [tptr tvoid]
-    EX q: val, EX k: oi.(key), EX v: oi.(value), EX r: val,
-    PROP()
-    LOCAL(temp ret_temp r)
-    SEP(oi.(kvpair_repr) sh (k, v) q * oi.(cursor_repr) (fst mc, snd mc + 1) r).
-         (* how to represent the case where cursor is null ? can we just have a null pointer? *)
-
-(* move_to_next don't change the cursor if you're at the end *)
-
-
-Definition get_previous_spec 
-  (oi: OrderedIndex.index): funspec :=
-  WITH sh: share, p: val, mc: oi.(cursor)
-  PRE [ 1%positive OF tptr tvoid]
-    PROP()
-    LOCAL( temp 1%positive p)
-    SEP(oi.(cursor_repr) mc p)
-  POST [tptr tvoid]
-    EX q: val, EX k: oi.(key), EX v: oi.(value), EX r: val,
-    PROP()
-    LOCAL(temp ret_temp r)
-    SEP(oi.(kvpair_repr) sh (k, v) q * oi.(cursor_repr) (fst mc, snd mc - 1) r). *)
+    SEP(mem_mgr gv; oi.(t_repr) sh m p *  oi.(key_repr) sh k q *oi.(cursor_repr) c r). *)
 
 (* takes t, returns cursor pointing to 0 *)
 Definition move_to_first_spec 
   (oi: OrderedIndex.index): funspec :=
-  WITH gv: globals, sh: share, p: val, m: oi.(t)
+  WITH gv: globals, sh: share, p: val, cur: oi.(cursor), numrec: Z
+  PRE [ 1%positive OF tptr oi.(cursor_type)]
+    PROP()
+    LOCAL( temp 1%positive p)
+    SEP(mem_mgr gv; oi.(cursor_repr) cur p numrec)
+  POST [tint]
+    PROP()
+    LOCAL(temp ret_temp (Val.of_bool (oi.(valid_cursor) (oi.(move_to_first) cur))))
+    SEP(mem_mgr gv; oi.(cursor_repr) (oi.(move_to_first) cur) p numrec).
+
+
+
+Definition move_to_previous_spec 
+  (oi: OrderedIndex.index): funspec :=
+  WITH gv: globals, sh: share, p: val, cur: oi.(cursor), numrec: Z
   PRE [ 1%positive OF tptr tvoid]
     PROP()
     LOCAL( temp 1%positive p)
-    SEP(mem_mgr gv; oi.(t_repr) sh m p)
+    SEP(mem_mgr gv; oi.(cursor_repr) cur p numrec)
   POST [tptr tvoid]
     EX r: val,
     PROP()
     LOCAL(temp ret_temp r)
-    SEP(mem_mgr gv; oi.(t_repr) sh m p *  oi.(cursor_repr) (m, 0) r).
+    SEP(mem_mgr gv; oi.(cursor_repr) (oi.(move_to_previous) cur) p numrec).
 
-(* takes t, returns cursor pointing to last *)
 Definition move_to_last_spec 
   (oi: OrderedIndex.index): funspec :=
-  WITH gv: globals, sh: share, p: val, m: oi.(t)
+  WITH gv: globals, sh: share, p: val, cur: oi.(cursor), numrec: Z
   PRE [ 1%positive OF tptr tvoid]
     PROP()
     LOCAL( temp 1%positive p)
-    SEP(mem_mgr gv; oi.(t_repr) sh m p)
+    SEP(mem_mgr gv; oi.(cursor_repr) cur p numrec)
   POST [tptr tvoid]
     EX r: val,
     PROP()
     LOCAL(temp ret_temp r)
-    SEP(mem_mgr gv; oi.(t_repr) sh m p *  oi.(cursor_repr) (m, (Zlength (elements (oi.(flatten) m))-1)) r).
+    SEP(mem_mgr gv; oi.(cursor_repr) (oi.(move_to_last) cur) p numrec).
 
-(* takes cursor, kvpair, returns cursor *)
 (*
-Definition insert_spec 
-  (oi: OrderedIndex.index): funspec :=
-  WITH sh: share, p: val, q: val, mc: oi.(cursor), kv: oi.(kvpair)
-  PRE [ 1%positive OF tptr tvoid, 2%positive OF tptr tvoid]
-    PROP()
-    LOCAL( temp 1%positive p; temp 2%positive q)
-    SEP(oi.(cursor_repr) mc p *  oi.(kvpair_repr) sh kv q)
-  POST [tptr tvoid]
-    EX c: Z, EX r: val,
-    PROP()
-    LOCAL(temp ret_temp r)
-    SEP(oi.(cursor_repr) (fst mc, c) r *  oi.(kvpair_repr) sh kv q). *)
-(* use flat to represent insertion, calculate new cursor using get cursor *)
-
-(* takes cursor, key, returns cursor *)
-(*
-Definition delete_spec 
-  (oi: OrderedIndex.index): funspec :=
-  WITH sh: share, p: val, q: val, mc: oi.(cursor), kv: oi.(kvpair)
-  PRE [ 1%positive OF tptr tvoid, 2%positive OF tptr tvoid]
-    PROP()
-    LOCAL( temp 1%positive p; temp 2%positive q)
-    SEP(oi.(cursor_repr) mc p *  oi.(kvpair_repr) sh kv q)
-  POST [tptr tvoid]
-    EX c: Z, EX r: val,
-    PROP()
-    LOCAL(temp ret_temp r)
-    SEP(oi.(cursor_repr) (fst mc, c) r). *)
-
 Definition lookup_spec 
   (oi: OrderedIndex.index): funspec :=
-  WITH sh: share, p: val, q: val, m: oi.(t), k: oi.(key)
-  PRE [ 1%positive OF tptr tvoid, 2%positive OF tptr tvoid]
+  WITH gv: globals, sh: share, p: val, q: val, m: oi.(t), k: oi.(key)
+  PRE [ 1 OF tptr tvoid, 2 OF tptr tvoid]
     PROP()
-    LOCAL( temp 1%positive p; temp 2%positive q)
-    SEP(oi.(t_repr) sh m p *  oi.(key_repr) sh k q)
+    LOCAL( temp 1 p; temp 2 q)
+    SEP(mem_mgr gv; oi.(t_repr) sh m p *  oi.(key_repr) sh k q)
   POST [tptr tvoid]
     PROP()
     LOCAL(temp ret_temp (proj1_sig (oi.(lookup) m k)))
-    SEP(oi.(t_repr) sh m p *  oi.(key_repr) sh k q).
+    SEP(mem_mgr gv; oi.(t_repr) sh m p * oi.(key_repr) sh k q).
 
-(* flatten? *)
+(* spec does not allow inserting into null structure *)
+Definition insert_spec 
+  (oi: OrderedIndex.index): funspec :=
+  WITH gv: globals, sh: share, mptr: val, kptr: val, m: oi.(t), k: oi.(key), v: V
+  PRE [ 1%positive OF tptr tvoid, 2%positive OF tptr tvoid, 3%positive OF tptr tvoid]
+    PROP()
+    LOCAL(gvars gv; temp 1%positive mptr; temp 2%positive kptr; temp 3%positive (V_repr v))
+    SEP(mem_mgr gv; oi.(t_repr) sh m mptr *  oi.(key_repr) sh k kptr)
+  POST [tptr tvoid]
+    EX newm: oi.(t),
+    PROP( oi.(lookup) newm k = v)
+    LOCAL(temp ret_temp (proj1_sig (oi.(lookup) m k)))
+    SEP(mem_mgr gv; oi.(t_repr) sh newm mptr * oi.(key_repr) sh k kptr).
+
+*)
 
 End OrderedIndex.
