verif/indices/stringlist_instance.v
@@ -61,7 +61,7 @@ Definition stringlist_index : index :=
      
      create := stringlist_model.empty V;
 
-     cursor_repr := fun mc p => emp;
+     cursor_repr := fun mc p => stringlist_cursor_rep mc p;
 
      flatten := fun lst => mk_flat _  (stringlist_model.elements (elt:=V) lst) (lstnodup lst);
      
@@ -87,9 +87,19 @@ Definition exit_spec := (_exit, exit_funspec).
 Definition cardinality_funspec := cardinality_spec(stringlist_index).
 Definition stringlist_cardinality_spec := (_stringlist_cardinality, cardinality_funspec).
 
+Definition move_to_first_funspec := move_to_first_spec(stringlist_index).
+Definition stringlist_move_to_first_spec := (_stringlist_move_to_first, move_to_first_funspec).
+
+Definition move_to_next_funspec := move_to_next_spec(stringlist_index).
+Definition stringlist_move_to_next_spec := (_stringlist_move_to_next, move_to_next_funspec).
+
+Definition get_cursor_funspec := get_cursor_spec(stringlist_index).
+Definition stringlist_get_cursor_spec := (_stringlist_get_cursor, get_cursor_funspec).
+
 Definition Gprog : funspecs := [ new_scell_spec; strcmp_spec; malloc_spec;
     exit_spec; stringlist_create_spec; stringlist_lookup_spec; stringlist_insert_spec;
-    stringlist_cardinality_spec ].
+    stringlist_cardinality_spec; stringlist_move_to_first_spec;
+    stringlist_move_to_next_spec; stringlist_get_cursor_spec].
 
 (* ==================== HELPERS ==================== *)
 
@@ -209,17 +219,357 @@ Proof.
          symmetry in H2. contradiction.
 Qed.
 
+Lemma data_at_stringlist_ptr: forall cell_ptr p,
+  data_at Ews t_stringlist cell_ptr p |-- data_at Ews (tptr t_scell) cell_ptr p.
+Proof. 
+  intros. unfold_data_at (data_at _ _ _ p). rewrite field_at_data_at.
+  unfold field_address. if_tac; simpl; auto.
+  * entailer!.
+  * entailer!. apply field_compatible_isptr in H0. inversion H0.
+Qed.
+
+(* ==================== GET CURSOR ==================== *)
+
+Definition undef_cursor (p vret : val) : mpred :=
+  malloc_token Ews t_cursor vret * data_at Ews t_cursor (p, Vundef) vret. 
+
+Lemma body_stringlist_get_cursor: semax_body Vprog Gprog 
+    f_stringlist_get_cursor stringlist_get_cursor_spec.
+Proof.
+  unfold stringlist_get_cursor_spec. unfold get_cursor_funspec.
+  unfold get_cursor_spec. start_function.
+  simpl. Intros. forward. forward_call (t_cursor, gv).
+  { split; try auto; try omega. simpl. easy. }
+  { Intros vret. autorewrite with norm. 
+    forward_if (vret <> nullval). if_tac; entailer!.
+    { rewrite if_true by auto. forward_call tt. entailer!. }
+    { forward. entailer!. }
+    { Intros. rewrite if_false by auto. Intros. forward.
+      simpl. 
+      forward_loop 
+      (EX lst1: list (string * V), EX lst2: list (string * V), EX p0: val,
+      PROP( lst1 ++ lst2 = stringlist_model.elements m /\ 
+                not (stringlist_model.Raw.PX.In k lst1)) 
+      LOCAL(temp _mc vret; temp _cur (Vptrofs(Ptrofs.repr(Zlength(lst1)))); 
+                 gvars gv; temp _p p; temp _key q; temp _q p0)
+      SEP(mem_mgr gv;
+            stringlist_hole_rep lst2 m p p0 * string_rep k q *
+            undef_cursor p vret))
+      (* break cond *)
+      break: 
+      (EX lst2: list (string * V), EX p0: val, PROP ( )
+      LOCAL (temp _mc vret; temp _cur (Vlong (Int64.repr 0)); 
+                  gvars gv; temp _p p; temp _key q; temp _q p0)
+      SEP (mem_mgr gv; stringlist_hole_rep lst2 m p p0; 
+             string_rep k q; undef_cursor p vret)).
+      { unfold stringlist_rep. Intros cell_ptr. forward.
+        Exists (@nil (string * V)) (stringlist_model.elements m).
+        Exists cell_ptr.
+        unfold stringlist_hole_rep.
+        Exists cell_ptr. autorewrite with sublist. entailer!.
+        { inversion H8. inversion H9. }
+        { unfold undef_cursor.  cancel. apply wand_refl_cancel_right. }}
+      { Intros lst1 lst2 p0. forward_if (p0 <> nullval).
+        { unfold stringlist_hole_rep. Intros cell_ptr. entailer!. }
+        { forward. entailer!. }
+        { forward. Exists lst2 p0. entailer!. admit. }
+        { destruct lst2.
+          { unfold stringlist_hole_rep. Intros cell_ptr.
+            unfold scell_rep; fold scell_rep. Intros. contradiction. }
+          { unfold stringlist_hole_rep. Intros cell_ptr. destruct p1.
+            unfold scell_rep at 1; fold scell_rep. Intros q0 str_ptr.
+            forward. 
+            forward_call (str_ptr, string_to_list_byte s, q, string_to_list_byte k).
+            { unfold cstring. unfold string_rep.
+              repeat rewrite length_string_list_byte_eq. cancel. }
+            Intros vret0. forward_if. destruct Int.eq_dec in H3.
+            { unfold undef_cursor. Intros. forward. forward.
+              Exists vret. unfold cursor. Exists (m, 0). entailer!.
+              simpl t_repr. simpl key_repr. simpl cursor_repr.
+              unfold string_rep. unfold cstring at 2. repeat rewrite length_string_list_byte_eq.
+              cancel. unfold stringlist_rep. Exists cell_ptr. cancel.
+              unfold stringlist_cursor_rep. Exists p. cancel.
+              apply wand_sepcon_adjoint.
+              assert (K: cstring Ews (string_to_list_byte s) str_ptr * malloc_token Ews t_scell p0 *
+                 data_at Ews t_scell (str_ptr, (V_repr v, q0)) p0 *
+                 malloc_token Ews (tarray tschar (Zlength (string_to_list_byte s) + 1)) str_ptr *
+                 scell_rep lst2 q0 |-- 
+                 scell_rep ((s, v) :: lst2) p0).
+                 { unfold scell_rep at 2; fold scell_rep. Exists q0 str_ptr.
+                   unfold cstring. unfold string_rep. rewrite length_string_list_byte_eq.
+                   cancel. }
+              sep_apply K. apply wand_sepcon_adjoint. admit. 
+              (* apply modus_ponens_wand. *) }
+            { unfold not in n. contradiction. }
+            { forward. forward. Exists (lst1 ++ [(s, v)]) lst2. Exists q0.
+              entailer!. 
+              { repeat split. 
+                 { rewrite <- H0. rewrite app_assoc_reverse. simpl. auto. }
+                 { destruct (Int.eq_dec vret0 Int.zero) in H3.
+                   contradiction. unfold not. intros. unfold stringlist_model.Raw.PX.In in H15. 
+                   unfold stringlist_model.Raw.PX.In in H1. unfold not in H1.
+                   unfold stringlist_model.Raw.PX.MapsTo in H15. inversion H15. 
+                   rewrite SetoidList.InA_app_iff in H16. inversion H16.
+                   { unfold stringlist_model.Raw.PX.MapsTo in H1. apply H1. exists x. auto. }
+                   { inversion H17. inversion H19. simpl in H21. rewrite H21 in H3. 
+                      contradiction. inversion H19. }}
+                   { admit. }}
+               { admit. }}}}}
+      { Intros lst2 p0. unfold undef_cursor. Intros. forward. forward.
+        Exists vret (m, 0). entailer!. simpl. cancel. unfold stringlist_cursor_rep.
+        Exists p. cancel. unfold stringlist_hole_rep. Intros cell_ptr.
+        unfold stringlist_rep at 1. Exists cell_ptr. cancel. admit.
+        (* apply modus_ponens_wand. *)  } 
+
+(* need to fix the double definition of stringlist and also the cursor number *)
+Admitted.
+
+
+
+(* ==================== MOVE TO NEXT ==================== *)
+
+Lemma body_stringlist_move_to_next: semax_body Vprog Gprog 
+    f_stringlist_move_to_next stringlist_move_to_next_spec.
+Proof. 
+  unfold stringlist_move_to_next_spec. unfold move_to_next_funspec.
+  unfold move_to_next_spec. start_function. 
+  forward. simpl. unfold stringlist_cursor_rep. Intros strlst_p.
+  sep_apply stringlist_rep_local_facts.
+  simpl. forward.
+  forward. forward_call (sh, strlst_p, m).
+    { simpl. entailer!. }
+    { forward. autorewrite with norm.
+      remember (Int64.repr (prevcur + 1)) as nextcur.
+      remember (Int64.repr (Zlength (elements (flatten stringlist_index m)))) as length.
+      remember (Int64.ltu nextcur length) as cond1.
+      remember (Int64.ltu (Int64.repr 0) nextcur) as cond2.
+      remember (andb cond1 cond2) as condition.
+      forward_if
+        (PROP ( )
+        LOCAL (temp _cur (Vlong nextcur);
+                    temp _length (Vlong length); temp _lst strlst_p; 
+                    temp _mc p; temp _mcc p; temp _t'2 (if condition then Vtrue else Vfalse))
+        SEP (t_repr stringlist_index sh m strlst_p; mem_mgr gv;
+               malloc_token Ews t_cursor p;
+               data_at Ews t_cursor (strlst_p, Vlong (Int64.repr prevcur)) p)).
+      { forward. entailer!. unfold cardinality in H.
+        rewrite H. simpl. unfold Val.of_bool. auto. }
+      { forward. entailer!. unfold cardinality in H. rewrite H. simpl. auto. }
+      { forward_if
+        (PROP ( )
+        LOCAL (temp _cur (Vlong nextcur); temp _length (Vlong length);
+                    temp _lst strlst_p; temp _mc p; temp _mcc p;
+                    temp _t'2 (if condition then Vtrue else Vfalse))
+        SEP (mem_mgr gv;
+         cursor_repr stringlist_index
+           (move_to_next stringlist_index (m, prevcur)) p)).
+      destruct condition.
+        { forward. entailer!.
+          assert (K: (move_to_next stringlist_index (m, prevcur)) = (m, prevcur+1)).
+          { simpl in *. rewrite <- Heqcondition. auto. }
+          rewrite K. simpl. unfold stringlist_cursor_rep.
+          Exists strlst_p. entailer!. }
+        { inversion H. }
+        { forward. entailer!. 
+          assert (K: (move_to_next stringlist_index (m, prevcur)) = (m, 0)).
+          { simpl in *. rewrite H. auto. }
+          rewrite K. simpl. unfold stringlist_cursor_rep.
+          Exists strlst_p. entailer!. } 
+       forward. Exists p. entailer!. }}
+Qed.
+
+
+(* ==================== MOVE TO FIRST ==================== *)
+
+Lemma body_stringlist_move_to_first: semax_body Vprog Gprog 
+    f_stringlist_move_to_first stringlist_move_to_first_spec.
+Proof. 
+  unfold stringlist_move_to_first_spec. unfold move_to_first_funspec.
+  unfold move_to_first_spec. start_function. 
+  forward. simpl. unfold stringlist_cursor_rep. Intros strlst_p.
+  simpl.
+  forward. forward. Exists p. simpl. unfold stringlist_cursor_rep.
+  entailer!. Exists strlst_p. simpl. entailer!.
+Qed.
+
+
 (* ================== CARDINALITY ================== *)
 
-(*Ltac check_parameter_vals Delta al ::= idtac. *)
 
 Lemma body_stringlist_cardinality: semax_body Vprog Gprog 
     f_stringlist_cardinality stringlist_cardinality_spec.
 Proof. 
   unfold stringlist_cardinality_spec. unfold cardinality_funspec.
-  unfold cardinality_spec. start_function.
+  unfold cardinality_spec. start_function. 
+  forward. simpl. unfold stringlist_rep. Intros cell_ptr.
+  simpl in m.  
+  (* invariant *)
+   forward_loop 
+  (EX lst1: list (string * V), EX lst2: list (string * V), EX p0: val,
+  PROP( lst1 ++ lst2 = stringlist_model.elements m) 
+  LOCAL(temp _q p0; temp _size (Vptrofs (Ptrofs.repr (Zlength(lst1)))); temp _p p)
+  SEP(stringlist_hole_rep lst2 m p p0))
+  (* break cond *)
+  break: 
+  (PROP () 
+  LOCAL(temp _size (Vptrofs (Ptrofs.repr (Zlength(stringlist_model.elements m)))))
+  SEP((stringlist_rep m p))).
+  (* holds on entry *)
+  - forward.
+     Exists (@nil (string * V)) (stringlist_model.elements m) cell_ptr.
+     entailer!. unfold stringlist_hole_rep. Exists cell_ptr. entailer!.
+     apply wand_refl_cancel_right.
+  (* holds on iteration *)
+  - Intros lst1 lst2 p0. unfold stringlist_hole_rep.
+     Intros cp0. forward_if (p0 <> nullval).
+     { forward. entailer!. }
+     { forward. autorewrite with norm. 
+       entailer!.
+       { assert (K: nullval = nullval) by auto.  apply H4 in K.
+         subst. rewrite <- H. autorewrite with sublist. auto. }
+       unfold stringlist_rep. Exists cp0.
+       cancel. apply modus_ponens_wand. }
+      { forward. autorewrite with norm. destruct lst2.
+        (* lst2 empty *)
+       { unfold scell_rep; fold scell_rep. Intros. contradiction. }
+         (* lst2 not empty *)
+       { destruct p1.
+         unfold scell_rep at 1; fold scell_rep. Intros q0 str_ptr.
+         forward. entailer!.
+         Exists (lst1 ++ [(s,v)]) lst2 q0. entailer!.
+         split.
+         { rewrite app_assoc_reverse. simpl. auto. }
+         { f_equal. f_equal. rewrite Zlength_app. easy. }
+         unfold stringlist_hole_rep. Exists cp0. 
+         entailer!. apply wand_frame_intro'.
+         apply wand_sepcon_adjoint. apply wand_frame_intro'.
+         assert (W: malloc_token Ews t_scell p0 * 
+                         data_at Ews t_scell (str_ptr, (V_repr v, q0)) p0 *
+                         string_rep s str_ptr *
+                         malloc_token Ews (tarray tschar (Z.of_nat (length s) + 1)) str_ptr * 
+                         scell_rep lst2 q0 |-- scell_rep ((s, v) :: lst2) p0).
+         { unfold scell_rep at 2; fold scell_rep. Exists q0 str_ptr. cancel. }
+         sep_apply W. sep_apply modus_ponens_wand. cancel. }}
+ - autorewrite with norm. forward. 
+Qed.
 
-Admitted.
+
+
+(* ==================== LOOKUP ==================== *)
+
+Lemma body_stringlist_lookup: semax_body Vprog Gprog 
+    f_stringlist_lookup stringlist_lookup_spec.
+Proof. unfold stringlist_lookup_spec. unfold lookup_funspec. unfold lookup_spec.
+  start_function. simpl. remember m as lst. remember k as str.
+  (* loop invariant *)
+  forward_loop 
+  (EX lst1: list (string * V), EX lst2: list (string * V), EX p0: val,
+  PROP( lst1 ++ lst2 = stringlist_model.elements lst /\ not (stringlist_model.Raw.PX.In str lst1)) 
+  LOCAL(temp _q p0; temp _key q)
+  SEP(mem_mgr gv; stringlist_hole_rep lst2 lst p p0 * string_rep str q))
+  (* break cond *)
+  break: 
+  (PROP (nullval = proj1_sig (lookup stringlist_index m k)) 
+  LOCAL()
+  SEP((mem_mgr gv * stringlist_rep lst p * string_rep str q))).
+ (* invariant holds entering loop*) 
+  - unfold stringlist_rep. Intros cell_ptr. forward. 
+     Exists (@nil (string * V)) (stringlist_model.elements lst).
+     Exists cell_ptr.
+     unfold stringlist_hole_rep.
+     Exists cell_ptr. autorewrite with sublist. entailer!.
+     { inversion H4. inversion H5. }
+     { apply wand_refl_cancel_right. }
+  (* invariant holds in the loop *)
+  - Intros lst1 lst2 p0. forward_if (p0 <> nullval).
+    { unfold stringlist_hole_rep. Intros cell_ptr. entailer!. }
+    { forward. entailer!. }
+    { (* break inv used *) unfold stringlist_hole_rep. Intros cell_ptr.
+      rewrite H1.  forward. entailer!.
+      { assert (K: nullval = nullval). auto. apply H5 in K. 
+        subst. autorewrite with sublist in H.
+        rewrite H in H0. replace (lookup stringlist_index m k) with nullV; auto.
+        unfold lookup. simpl. simpl in k. simpl in m. apply notin_lst_find_none in H0.
+        assert 
+        (P: @find stringlist_model.key V Str_as_DT.eq_dec (stringlist_model.elements (elt:=V) m) k = None).
+        { rewrite <- H0.
+          apply stringlistfind_eq_find. }
+          rewrite P; auto. }
+        { unfold stringlist_rep. Exists cell_ptr. cancel.
+         apply modus_ponens_wand. }}
+    { destruct lst2. 
+        (* lst2 empty *)
+       { unfold stringlist_hole_rep. Intros cell_ptr.
+         unfold scell_rep; fold scell_rep. Intros. contradiction. }
+         (* lst2 not empty *)
+       { unfold stringlist_hole_rep. Intros cell_ptr. destruct p1.
+         unfold scell_rep at 1; fold scell_rep. Intros q0 str_ptr.
+         forward. 
+         forward_call (str_ptr, string_to_list_byte s, q, string_to_list_byte str).
+         { unfold cstring. unfold string_rep.
+           repeat rewrite length_string_list_byte_eq. cancel. }
+         Intros vret. forward_if.
+         { destruct (Int.eq_dec vret Int.zero) in H2.
+           { forward.
+              { unfold V in v. entailer!.
+                destruct v. auto. }
+              { forward. entailer!.
+                { assert (M: lookup stringlist_index m k = v).
+                  { apply list_byte_eq in H2; rewrite <- H2. unfold lookup. simpl in k. simpl in m.
+                    assert (K: stringlist_model.elements m = (elements (flatten stringlist_index m))) by auto.
+                    rewrite <- K. rewrite <- H. simpl.
+                    assert 
+                    (P: @find stringlist_model.key V Str_as_DT.eq_dec (lst1 ++ (s, v) :: lst2) s 
+                     = (Some v)).
+                    { assert (W: NoDup (map fst (stringlist_model.elements (elt:=V) m))).
+                      apply lstnodup. rewrite <- H in W. rewrite map_app in W. simpl in W. 
+                      apply (@NoDup_remove_2 string (map fst (lst1)) (map fst (lst2)) s) in W.
+                      apply find_middle; auto. }
+                    rewrite P. auto. } rewrite M; simpl; auto. } 
+                 simpl t_repr. simpl key_repr. unfold string_rep. unfold cstring at 2. rewrite length_string_list_byte_eq.
+                 cancel. unfold stringlist_rep. Exists cell_ptr. cancel.
+                 apply wand_sepcon_adjoint.
+                 assert (K: cstring Ews (string_to_list_byte s) str_ptr * malloc_token Ews t_scell p0 *
+                 data_at Ews t_scell (str_ptr, (V_repr v, q0)) p0 *
+                 malloc_token Ews (tarray tschar (Zlength (string_to_list_byte s) + 1)) str_ptr *
+                 scell_rep lst2 q0 |-- 
+                 scell_rep ((s, v) :: lst2) p0).
+                 { unfold scell_rep at 2; fold scell_rep. Exists q0 str_ptr.
+                   unfold cstring. unfold string_rep. rewrite length_string_list_byte_eq.
+                   cancel. }
+                  sep_apply K. apply wand_sepcon_adjoint. apply modus_ponens_wand. }}
+           { contradiction. }}
+          { destruct (Int.eq_dec vret Int.zero) in H2.
+            contradiction.
+            abbreviate_semax. forward. Exists (lst1 ++ [(s, v)]) lst2.
+            Exists q0. entailer!.
+            { split.
+              { rewrite <- H. rewrite app_assoc_reverse. simpl. auto. }
+              { unfold not. intros. unfold stringlist_model.Raw.PX.In in H14. 
+                unfold stringlist_model.Raw.PX.In in H0. unfold not in H0.
+                unfold stringlist_model.Raw.PX.MapsTo in H14. inversion H14. 
+                rewrite SetoidList.InA_app_iff in H15. inversion H15.
+                { unfold stringlist_model.Raw.PX.MapsTo in H0. apply H0. exists x. auto. }
+                { inversion H16. inversion H18. simpl in H20. rewrite H20 in H2. 
+                  contradiction. inversion H18. }}}
+             { unfold string_rep. unfold cstring at 2. rewrite length_string_list_byte_eq.
+               cancel. unfold stringlist_hole_rep. Exists cell_ptr. 
+               entailer!. apply wand_frame_intro'.
+               apply wand_sepcon_adjoint. apply wand_frame_intro'.
+               assert (K: cstring Ews (string_to_list_byte s) str_ptr * malloc_token Ews t_scell p0 *
+               data_at Ews t_scell (str_ptr, (V_repr v, q0)) p0 *
+               malloc_token Ews (tarray tschar (Zlength (string_to_list_byte s) + 1)) str_ptr * 
+               scell_rep lst2 q0 |-- 
+               scell_rep ((s, v) :: lst2) p0).
+               { unfold scell_rep at 2; fold scell_rep. Exists q0 str_ptr.
+                 unfold cstring. unfold string_rep. rewrite length_string_list_byte_eq.
+                 cancel. }
+               sep_apply K. apply modus_ponens_wand. }}}}
+  (* invariant holds after loop *) (* break inv used *)
+  - forward. entailer!. simpl. auto. 
+Qed.
+  
+
 
 
 
@@ -249,7 +599,7 @@ Qed.
 
 (* ==================== INSERT ==================== *)
 
-(* 
+
 Lemma body_stringlist_insert: semax_body Vprog Gprog 
     f_stringlist_insert stringlist_insert_spec.
 Proof. 
@@ -377,8 +727,8 @@ Proof.
                 unfold stringlist_model.Raw.elements in H. clear M. clear P. clear H3. 
                 rewrite <- H.
                 apply notin_lst_add_middle. auto. }}
-              { forward. entailer!. 
-                Exists (lst1 ++ [(k0,v0)]) lst2 (offset_val 8 cellptr2) q. entailer!.
+              { forward. entailer!.
+                Exists (lst1 ++ [(k0,v0)]) lst2 (offset_val 16 cellptr2) q. entailer!.
                 { split.
                   * rewrite app_assoc_reverse. simpl. rewrite H. auto.
                   * apply notin_cons. auto. destruct (Int.eq_dec vret Int.zero).
@@ -401,7 +751,7 @@ Proof.
                 (tarray tschar (Zlength (string_to_list_byte k0) + 1)) str_ptr * 
                 (field_at Ews t_scell [StructField _value] (V_repr v0) cellptr2 *
                 data_at Ews (tptr t_scell) cellptr2 addr))))) *
-                strlst_rep (offset_val 8 cellptr2) cpnew lst' |-- strlst_rep addr cellptr2 ((k0, v0) :: lst')).
+                strlst_rep (offset_val 16 cellptr2) cpnew lst' |-- strlst_rep addr cellptr2 ((k0, v0) :: lst')).
                 { unfold strlst_rep. cancel. unfold scell_rep at 2; fold scell_rep.
                   Exists cpnew str_ptr. cancel.
                   unfold cstring. unfold string_rep.
@@ -412,118 +762,4 @@ Proof.
                 rewrite app_assoc_reverse. simpl. entailer!. }}
 Qed.
 
-*)
 
-(* ==================== LOOKUP ==================== *)
-
-Lemma body_stringlist_lookup: semax_body Vprog Gprog 
-    f_stringlist_lookup stringlist_lookup_spec.
-Proof. unfold stringlist_lookup_spec. unfold lookup_funspec. unfold lookup_spec.
-  start_function. simpl. remember m as lst. remember k as str.
-  (* loop invariant *)
-  forward_loop 
-  (EX lst1: list (string * V), EX lst2: list (string * V), EX p0: val,
-  PROP( lst1 ++ lst2 = stringlist_model.elements lst /\ not (stringlist_model.Raw.PX.In str lst1)) 
-  LOCAL(temp _q p0; temp _key q)
-  SEP(mem_mgr gv; stringlist_hole_rep lst2 lst p p0 * string_rep str q))
-  (* break cond *)
-  break: 
-  (PROP (Vint (Int.repr 0) = proj1_sig (lookup stringlist_index m k)) 
-  LOCAL()
-  SEP((mem_mgr gv * stringlist_rep lst p * string_rep str q))).
- (* invariant holds entering loop*) 
-  - unfold stringlist_rep. Intros cell_ptr. forward. 
-     Exists (@nil (string * V)) (stringlist_model.elements lst).
-     Exists cell_ptr.
-     unfold stringlist_hole_rep.
-     Exists cell_ptr. autorewrite with sublist. entailer!.
-     { inversion H4. inversion H5. }
-     { apply wand_refl_cancel_right. }
-  (* invariant holds in the loop *)
-  - Intros lst1 lst2 p0. forward_if (p0 <> nullval).
-    { unfold stringlist_hole_rep. Intros cell_ptr. entailer!. }
-    { forward. entailer!. }
-    { (* break inv used *) unfold stringlist_hole_rep. Intros cell_ptr.
-      rewrite H1.  forward. entailer!.
-      { assert (K: nullval = nullval). auto. apply H5 in K. 
-        subst. autorewrite with sublist in H.
-        rewrite H in H0. replace (lookup stringlist_index m k) with nullV; auto.
-        unfold lookup. simpl. simpl in k. simpl in m. apply notin_lst_find_none in H0.
-        assert 
-        (P: @find stringlist_model.key V Str_as_DT.eq_dec (stringlist_model.elements (elt:=V) m) k = None).
-        { rewrite <- H0.
-          apply stringlistfind_eq_find. }
-          rewrite P; auto. }
-        { unfold stringlist_rep. Exists cell_ptr. cancel.
-         apply modus_ponens_wand. }}
-    { destruct lst2. 
-        (* lst2 empty *)
-       { unfold stringlist_hole_rep. Intros cell_ptr.
-         unfold scell_rep; fold scell_rep. Intros. contradiction. }
-         (* lst2 not empty *)
-       { unfold stringlist_hole_rep. Intros cell_ptr. destruct p1.
-         unfold scell_rep at 1; fold scell_rep. Intros q0 str_ptr.
-         forward. 
-         forward_call (str_ptr, string_to_list_byte s, q, string_to_list_byte str).
-         { unfold cstring. unfold string_rep.
-           repeat rewrite length_string_list_byte_eq. cancel. }
-         Intros vret. forward_if.
-         { destruct (Int.eq_dec vret Int.zero) in H2.
-           { forward.
-              { unfold V in v. entailer!.
-                destruct v. auto. }
-              { forward. entailer!.
-                { assert (M: lookup stringlist_index m k = v).
-                  { apply list_byte_eq in H2; rewrite <- H2. unfold lookup. simpl in k. simpl in m.
-                    assert (K: stringlist_model.elements m = (elements (flatten stringlist_index m))) by auto.
-                    rewrite <- K. rewrite <- H. simpl.
-                    assert 
-                    (P: @find stringlist_model.key V Str_as_DT.eq_dec (lst1 ++ (s, v) :: lst2) s 
-                     = (Some v)).
-                    { assert (W: NoDup (map fst (stringlist_model.elements (elt:=V) m))).
-                      apply lstnodup. rewrite <- H in W. rewrite map_app in W. simpl in W. 
-                      apply (@NoDup_remove_2 string (map fst (lst1)) (map fst (lst2)) s) in W.
-                      apply find_middle; auto. }
-                    rewrite P. auto. } rewrite M; simpl; auto. } 
-                 simpl t_repr. simpl key_repr. unfold string_rep. unfold cstring at 2. rewrite length_string_list_byte_eq.
-                 cancel. unfold stringlist_rep. Exists cell_ptr. cancel.
-                 apply wand_sepcon_adjoint.
-                 assert (K: cstring Ews (string_to_list_byte s) str_ptr * malloc_token Ews t_scell p0 *
-                 data_at Ews t_scell (str_ptr, (V_repr v, q0)) p0 *
-                 malloc_token Ews (tarray tschar (Zlength (string_to_list_byte s) + 1)) str_ptr *
-                 scell_rep lst2 q0 |-- 
-                 scell_rep ((s, v) :: lst2) p0).
-                 { unfold scell_rep at 2; fold scell_rep. Exists q0 str_ptr.
-                   unfold cstring. unfold string_rep. rewrite length_string_list_byte_eq.
-                   cancel. }
-                  sep_apply K. apply wand_sepcon_adjoint. apply modus_ponens_wand. }}
-           { contradiction. }}
-          { destruct (Int.eq_dec vret Int.zero) in H2.
-            contradiction.
-            abbreviate_semax. forward. Exists (lst1 ++ [(s, v)]) lst2.
-            Exists q0. entailer!.
-            { split.
-              { rewrite <- H. rewrite app_assoc_reverse. simpl. auto. }
-              { unfold not. intros. unfold stringlist_model.Raw.PX.In in H14. 
-                unfold stringlist_model.Raw.PX.In in H0. unfold not in H0.
-                unfold stringlist_model.Raw.PX.MapsTo in H14. inversion H14. 
-                rewrite SetoidList.InA_app_iff in H15. inversion H15.
-                { unfold stringlist_model.Raw.PX.MapsTo in H0. apply H0. exists x. auto. }
-                { inversion H16. inversion H18. simpl in H20. rewrite H20 in H2. 
-                  contradiction. inversion H18. }}}
-             { unfold string_rep. unfold cstring at 2. rewrite length_string_list_byte_eq.
-               cancel. unfold stringlist_hole_rep. Exists cell_ptr. 
-               entailer!. apply wand_frame_intro'.
-               apply wand_sepcon_adjoint. apply wand_frame_intro'.
-               assert (K: cstring Ews (string_to_list_byte s) str_ptr * malloc_token Ews t_scell p0 *
-               data_at Ews t_scell (str_ptr, (V_repr v, q0)) p0 *
-               malloc_token Ews (tarray tschar (Zlength (string_to_list_byte s) + 1)) str_ptr * 
-               scell_rep lst2 q0 |-- 
-               scell_rep ((s, v) :: lst2) p0).
-               { unfold scell_rep at 2; fold scell_rep. Exists q0 str_ptr.
-                 unfold cstring. unfold string_rep. rewrite length_string_list_byte_eq.
-                 cancel. }
-               sep_apply K. apply modus_ponens_wand. }}}}
-  (* invariant holds after loop *) (* break inv used *)
-  - forward. entailer!. simpl. auto. 
-Qed.
