verif/indices/btree_instance.v
@@ -1,0 +1,110 @@
+Require Import VST.floyd.functional_base VST.floyd.proofauto.
+Require Import VST.floyd.library.
+Require Import indices.ordered_interface.
+Require Import indices.definitions.
+Require Import btrees.btrees.
+Require Import btrees.btrees_sep.
+Require Import btrees.btrees_spec. 
+Require Import indices.btree_wrappers.
+
+Import OrderedIndex.
+
+Definition bt_relation := btrees.relation val.
+Definition bt_cursor := btrees.cursor val.
+
+Definition btree_index : index :=
+  {| key := btrees.key;
+     key_repr := fun sh k p => data_at sh (tptr tvoid) (btrees_sep.key_repr k) p;
+
+     default_value := nullval;
+
+     t := relation val;
+
+     t_repr := fun sh m p => relation_rep m (get_depth m);
+
+     cursor := (bt_relation * bt_cursor)%type;
+
+     cursor_repr := fun '(m, c) p nr=> relation_rep m nr * cursor_rep c m p;
+     cursor_type := tcursor;
+
+     (* helper functions *)
+     valid_cursor := fun '(m, c) => if (isValid c m) then true else false;
+
+    (* interface functions *)
+
+     cardinality := fun m => get_depth m;
+
+     move_to_next := fun '(m, c) => (m, (RL_MoveToNext c m));
+
+     move_to_previous := fun '(m, c) => (m, (RL_MoveToPrevious c m));
+
+     move_to_key := fun '(m, c) k => let (n, p) := m in (m, moveToKey val n k c);
+
+     move_to_first := fun '(m, c) =>  let (n, p) := m in (m, moveToFirst n c (length c));
+
+     move_to_last := fun '(m, c) =>  let (n, p) := m in (m, moveToLast val n c (Zlength c));
+
+   |}.
+
+Lemma sub_move_to_next: funspec_sub (move_to_next_spec btree_index) 
+    (snd btrees_spec.RL_MoveToNext_spec).
+Proof. 
+  unfold move_to_next_spec. simpl snd.
+  apply NDsubsume_subsume.
+  split; extensionality x; reflexivity.
+  split3; auto.
+  { unfold cursor_type; simpl. (* names? *) admit. }
+  { intros [[[cur p] r] numrec].
+    Exists (p, (r, cur), numrec) emp.
+    rewrite !insert_SEP. Intros.
+    apply andp_right. 
+    entailer!. simpl. 
+    entailer!.
+    entailer!. admit.
+    unfold cursor_repr. simpl.
+    entailer!.
+Admitted.
+
+
+Lemma sub_move_to_first: funspec_sub (move_to_first_spec btree_index) 
+    (snd btree_wrappers.RL_MoveToFirst_spec).
+Proof. 
+  unfold move_to_first_spec. simpl snd. 
+  apply NDsubsume_subsume. 
+  split; extensionality x; reflexivity.
+  split3; auto.
+  { unfold cursor_type; simpl. (* names? *) admit. }
+  { admit. }
+Admitted.
+
+
+Lemma sub_move_to_last: funspec_sub (move_to_last_spec btree_index) 
+    (snd btrees_spec.moveToLast_spec).
+Proof.  
+  unfold move_to_last_spec. simpl snd.
+  apply NDsubsume_subsume. 
+  split; extensionality x; reflexivity.
+  split3; auto.
+  { admit. }
+  { admit. }
+Admitted.
+
+
+
+Lemma sub_move_to_prev: funspec_sub (move_to_previous_spec btree_index) 
+    (snd btrees_spec.RL_MoveToPrevious_spec).
+Proof. 
+  unfold move_to_previous_spec. simpl snd.
+  apply NDsubsume_subsume.
+  split; extensionality x; reflexivity.
+  split3; auto.
+  { admit. }
+  { admit. }
+Admitted.
+
+
+
+
+
+
+
